Update docker container; Fix Makefile; Update documentation; Simplify Login model with separate initial states for client and server

workspace/src/cat-fact-api/DY.CatFactAPI.Extraction.fst
@@ -11,7 +11,7 @@ open DY.CatFactAPI.Protocol
 let run () : traceful (option unit)  =
   let _ = IO.debug_print_string "************* Programm Output *************\n" in
   let client:principal = "Alice" in
-  let server:principal = "catfact.ninja" in
+  let server:principal = "Bob" in
 
   let*? comm_keys_ids_client, comm_keys_ids_server = initialize_communication_reqres (http_t web_types kv_types) client server in
   
